MCequiv: remove type arg from lam; rename typecheck; fix lam typecheck

Exercises/MCequivScript.sml
@@ -24,9 +24,8 @@ Datatype:
 	expr =  Lit bool | Equal expr expr
 		  | If expr expr expr
           | Apply expr expr
-          | Lam expr expr (* TODO maybe remove type (first expr) *)
+          | Lam expr
           | Var num
-          | TypeTag type
 End
 
 val _ = export_rewrites ["expr_size_def"]
@@ -46,7 +45,7 @@ Definition isAtom:
 	(isAtom (Lit _) ⇔ T) ∧
 (*	isAtom (Recfun _ _ _) ∧ *)
 	(isAtom (Var _) ⇔ T) ∧
-	(isAtom (Lam _ _) ⇔ T) ∧
+	(isAtom (Lam _) ⇔ T) ∧
 	(isAtom _ ⇔ F)
 End
 
@@ -82,44 +81,11 @@ Theorem non_var_not_isVar[simp]:
 	¬(isVar (Equal e1 e2)) ∧
 	¬(isVar (If e1 e2 e3)) ∧
 	¬(isVar (Apply e1 e2)) ∧
-	¬(isVar (Lam t e1)) ∧
+	¬(isVar (Lam e1)) ∧
 	¬(isVar (Lit b))
 Proof
 	rw[isVar]
 QED
-
-(*
-Definition M_step:
-	M_step (Plus (Num a) (Num b)) = Num (a + b) ∧
-	M_step (Plus (Num a) b) = Plus (Num a) (M_step b) ∧
-	M_step (Plus a b) = Plus (M_step a) b ∧
-	M_step (Minus (Num a) (Num b)) = Num (a - b) ∧
-	M_step (Minus (Num a) b) = Minus (Num a) (M_step b) ∧
-	M_step (Minus a b) = Minus (M_step a) b ∧
-	M_step (Less (Num a) (Num b)) = Lit (a < b) ∧
-	M_step (Less (Num a) b) = Less (Num a) (M_step b) ∧
-	M_step (Less a b) = Less (M_step a) b ∧
-	M_step (Equal (Num a) (Num b)) = Lit (a = b) ∧
-	M_step (Equal (Num a) b) = Equal (Num a) (M_step b) ∧
-	M_step (Equal a b) = Equal (M_step a) b ∧
-	M_step (Divide (Num a) (Num b)) = Num (a `div` b) ∧
-	M_step (Divide (Num a) b) = Divide (Num a) (M_step b) ∧
-	M_step (Divide a b) = Divide (M_step a) b ∧
-	M_step (If (Lit True) t e) = t ∧
-	M_step (If (Lit False) t e) = e ∧
-	M_step (If b t e) = If (M_step b) t e ∧
-		M_step (Apply rec@(Recfun _ _ f) e2)
-	  | isAtom e2 = f rec e2
-	  | otherwise = Apply rec (M_step e2)  ∧
-	M_step (Apply e1 e2) = Apply (M_step e1) e2
-End
-*)
-
-(*
-Definition freevar_cutoff:
-	freevar_cutoff = 10
-End
-*)
 
 
 Definition shift_up_one:
@@ -138,20 +104,17 @@ End
 Definition subst:
 	subst e1 e2 n = case e1 of
 		Lit b => Lit b
-	  | TypeTag t => TypeTag t
 	  | Equal a b => Equal (subst a e2 n) (subst b e2 n)
 	  | If g a b => If (subst g e2 n) (subst a e2 n) (subst b e2 n)
 	  | Apply a b => Apply (subst a e2 n) (subst b e2 n)
-	  | Lam t e => Lam t (subst e (shift_up_one e2) (n+1))
+	  | Lam e => Lam (subst e (shift_up_one e2) (n+1))
 	  | Var m => if (n = m) then e2 else (Var m)
 End
 
 (* (\x (\y. xy)) (Var 0) *)
 (* (\. (\. (Var 1) (Var 0)))) (Var 0) *)
-(* TODO:
-	2. check higher order abstract syntax *)
 
-Definition M_step:
+
 (*	M_step (Plus (Num a) (Num b)) = Num (a + b) ∧
 	M_step (Plus (Num a) b) = Plus (Num a) (M_step b) ∧
 	M_step (Plus a b) = Plus (M_step a) b ∧
@@ -166,36 +129,19 @@ Definition M_step:
 	M_step (Equal a b) = Equal (M_step a) b ∧
 	M_step (Divide (Num a) (Num b)) = Num (a `div` b) ∧
 	M_step (Divide (Num a) b) = Divide (Num a) (M_step b) ∧
-	M_step (Divide a b) = Divide (M_step a) b ∧ *)
-	M_step (Lit e) = Lit e ∧
-	M_step (Var v) = Var v ∧
-	M_step (Lam t e) = Lam t e ∧
-	M_step (TypeTag t) = (TypeTag t) ∧
-	M_step (Equal (Lit a) (Lit b)) = Lit (a = b) ∧
-	M_step (Equal (Lit a) b) = Equal (Lit a) (M_step b) ∧
-	M_step (Equal a b) = Equal (M_step a) b ∧
-	M_step (If (Lit True) t e) = t ∧
-	M_step (If (Lit False) t e) = e ∧
-	M_step (If b t e) = If (M_step b) t e ∧
-	(M_step (Apply (Lam t e) e2) =
-		if isAtom e2 then
-			shift_down_one_bounded (subst e (shift_up_one e2) 0)
-		else
-			Apply (Lam t e) (M_step e2))	∧
-	M_step (Apply e1 e2) = Apply (M_step e1) e2
+	M_step (Divide a b) = Divide (M_step a) b ∧
+*)
+
 (*	M_step (Apply rec@(Recfun _ _ f) e2)
 	  | isAtom e2 = f rec e2
 	  | otherwise = Apply rec (M_step e2)  ∧
 	M_step (Apply e1 e2) = Apply (M_step e1) e2
 *)
-End
-
 
 Inductive M_step_inductive:
 	(∀e. M_step_inductive (Lit e) (Lit e)) ∧
 	(∀v. M_step_inductive (Var v) (Var v)) ∧
-	(∀t e. M_step_inductive (Lam t e) (Lam t e)) ∧
-	(∀t. M_step_inductive (TypeTag t) (TypeTag t)) ∧
+	(∀e. M_step_inductive (Lam e) (Lam e)) ∧
 	(∀a b. M_step_inductive (Equal (Lit a) (Lit b)) (Lit (a = b))) ∧
 	(∀a b b'.
 		M_step_inductive b b'
@@ -208,13 +154,13 @@ Inductive M_step_inductive:
 	(∀b t e b'.
 		M_step_inductive b b'
 		⇒ M_step_inductive (If b t e) (If b' t e)) ∧
-	(∀t e e2.
+	(∀e e2.
 		isAtom e2
-		⇒ M_step_inductive (Apply (Lam t e) e2)
+		⇒ M_step_inductive (Apply (Lam e) e2)
 						   (shift_down_one_bounded (subst e (shift_up_one e2) 0))) ∧
-	(∀t e e2 e2'.
+	(∀e e2 e2'.
 		M_step_inductive e2 e2'
-		⇒ M_step_inductive (Apply (Lam t e) e2) (Apply (Lam t e) e2')) ∧
+		⇒ M_step_inductive (Apply (Lam e) e2) (Apply (Lam e) e2')) ∧
 	(∀e1 e2 e1'.
 		M_step_inductive e1 e1'
 		⇒ M_step_inductive (Apply e1 e2) (Apply e1' e2))
@@ -228,6 +174,7 @@ End
 	?e2'. e = ...
 *)
 
+(*
 Theorem M_step_equal_bool_or_equal:
 ∀e1 e2. (∃b. M_step (Equal e1 e2) = Lit b) ∨
 		(∃e2'. M_step (Equal e1 e2) = Equal e1 e2') ∨
@@ -236,6 +183,7 @@ Proof
 	ho_match_mp_tac M_step_ind >> rw[M_step] >>
 	Cases_on `e2` >> rw[M_step]
 QED
+*)
 
 (*
 Theorem equal_step_size:
@@ -261,12 +209,8 @@ Termination
 End
 *)
 
-(* need to progress + preservation *)
 
-(* expr -> SOME type *)
-Definition typeCheck:
 (*	typeCheck (Num n) = IntTy ∧ *)
-	(typeCheck Γ (Lit b) = SOME BoolTy) ∧
 (*	typeCheck (Plus e1 e2) = case (typeCheck e1, typeCheck e2) of
 	                           (IntTy, IntTy) -> IntTy
 	                           _ -> error "type error"
@@ -278,50 +222,34 @@ Definition typeCheck:
 	                           _ -> error "type error"
 	typeCheck (Less e1 e2) = case (typeCheck e1, typeCheck e2) of
 	                           (IntTy, IntTy) -> BoolTy
-	                           _ -> error "type error" *)
-	(typeCheck Γ (Equal e1 e2) = case (typeCheck Γ e1, typeCheck Γ e2) of
-	                        (*   (IntTy, IntTy) -> BoolTy *)
-	                         |  (SOME BoolTy, SOME BoolTy) => SOME BoolTy
-	                         |  _ => NONE (* error "type error" *)) ∧
-	(typeCheck Γ (If c t e) = case (typeCheck Γ c, typeCheck Γ t, typeCheck Γ e) of
-	   | (SOME BoolTy, tt, te) => if tt = te then tt else NONE (* error "Branches have different types" *)
-	   | _ => NONE (* error "if condition should be bool" *)) ∧
-	(typeCheck Γ (Apply e1 e2) = case (typeCheck Γ e1, typeCheck Γ e2) of
-	   | (SOME (FunTy t1 t2), SOME t1') => if t1 = t1' then (SOME t2)
-	                                  else NONE (* error "Argument doesn't match function" *)
-	   | _ => NONE) ∧ (* error "Can't apply a non-function" *)
-	(typeCheck Γ (Lam t e) = typeCheck Γ t) ∧ (* error "Function body doesn't match type signature" *)
-	(typeCheck Γ (Var n) = if (n < LENGTH Γ) then (SOME (EL n Γ)) else NONE) ∧
-	(typeCheck Γ (TypeTag t) = SOME t)
-End
+	                           _ -> error "type error"
+*)
 
-(* TODO: change name *)
-Inductive typeCheck_inductive:
-	(∀Γ b. typeCheck_inductive Γ (Lit b) BoolTy) ∧
-	(∀Γ t. typeCheck_inductive Γ (TypeTag t) t) ∧
-	(∀Γ n. (n < LENGTH Γ) ⇒ typeCheck_inductive Γ (Var n) (EL n Γ)) ∧
+Inductive typeChecking:
+	(∀Γ b. typeChecking Γ (Lit b) BoolTy) ∧
+	(∀Γ n. (n < LENGTH Γ) ⇒ typeChecking Γ (Var n) (EL n Γ)) ∧
 	(∀Γ e1 e2.
-	    (typeCheck_inductive Γ e1 BoolTy
-	     ⇒ typeCheck_inductive Γ e2 BoolTy
-		 ⇒ typeCheck_inductive Γ (Equal e1 e2) BoolTy) ∧
+	    typeChecking Γ e1 BoolTy ∧
+	     typeChecking Γ e2 BoolTy
+		 ⇒ typeChecking Γ (Equal e1 e2) BoolTy) ∧
 	(∀Γ b t e tt.
-	    typeCheck_inductive Γ b BoolTy
-	    ⇒ typeCheck_inductive Γ t tt
-	    ⇒ typeCheck_inductive Γ e tt
-		⇒ typeCheck_inductive Γ (If b t e) tt) ∧
-	(∀e1 e2 t1 t1' t2 Γ.
-		typeCheck_inductive Γ e1 (FunTy t1 t2)
-		⇒ typeCheck_inductive Γ e2 t1
-		⇒ typeCheck_inductive Γ (Apply e1 e2) t2) ∧
-	(∀e t t1 t2 Γ.
-		typeCheck_inductive Γ t (FunTy t1 t2)
-		⇒ typeCheck_inductive (* TODO: extend Γ and prove e has type t2 *)
-		⇒ typeCheck_inductive Γ (Lam t e) (FunTy t1 t2))
+	    typeChecking Γ b BoolTy ∧
+	    typeChecking Γ t tt ∧
+	    typeChecking Γ e tt
+		⇒ typeChecking Γ (If b t e) tt) ∧
+	(∀Γ e1 e2 t1 t2.
+		typeChecking Γ e1 (FunTy t1 t2) ∧
+		typeChecking Γ e2 t1
+		⇒ typeChecking Γ (Apply e1 e2) t2) ∧
+	(∀Γ e t1 t2.
+	    typeChecking (t1::Γ) e t2 (* extend Γ and prove e has type t2 *)
+		⇒ (typeChecking Γ (Lam e) (FunTy t1 t2)))
 End
 
 (* Γ, x:t1 |- s:t2 *)
 (* Γ |- \x. s : FunTy t1 t2 *)
 
+(*
 Theorem typeCheck_equal_bool_or_none:
 ∀Γ e1 e2.	typeCheck Γ (Equal e1 e2) = SOME BoolTy ∨
 			typeCheck Γ (Equal e1 e2) = NONE
@@ -329,17 +257,20 @@ Proof
 	rw[] >> Cases_on `typeCheck Γ e1` >> Cases_on `typeCheck Γ e2` >> gs[typeCheck]
 	>> Cases_on `x` >> gs[] >> Cases_on `x'` >> gs[]
 QED
+*)
 
+(*
 Theorem M_progress:
 	∀Γ e t. typeCheck Γ e = SOME t ⇒ isAtom e ∨ ∃e'. M_step e = e'
 Proof
 	rw[M_step]
 QED
+*)
 
-Theorem M_progress_2:
-	∀Γ e t. typeCheck_inductive Γ e t ⇒ isAtom e ∨ ∃e'. M_step e = e'
+Theorem M_progress:
+	∀Γ e t. typeChecking Γ e t ⇒ isAtom e ∨ ∃e'. M_step_inductive e = e'
 Proof
-	rw[M_step]
+	rw[M_step_inductive_rules]
 QED
 
 (*
@@ -382,12 +313,6 @@ Proof
 	Induct_on `M_step_inductive` >> gs[]
 QED
 
-Theorem typetag_m_step_typetag:
-	∀t e. M_step_inductive (TypeTag t) e ⇒ e = TypeTag t
-Proof
-	Induct_on `M_step_inductive` >> gs[]
-QED
-
 Theorem var_m_step_var:
 	∀n e. M_step_inductive (Var n) e ⇒ e = Var n
 Proof
@@ -395,7 +320,7 @@ Proof
 QED
 
 Theorem lam_m_step_lam:
-	∀t e e'. M_step_inductive (Lam t e) e' ⇒ e' = (Lam t e)
+	∀e e'. M_step_inductive (Lam e) e' ⇒ e' = (Lam e)
 Proof
 	Induct_on `M_step_inductive` >> gs[]
 QED
@@ -423,38 +348,57 @@ QED
 Theorem m_step_apply:
 	∀e1 e2 e.
 		M_step_inductive (Apply e1 e2) e
-			⇒ ((isAtom e2 ∧ ∃t le. e1 = Lam t le ∧ e = shift_down_one_bounded (subst le (shift_up_one e2) 0)) ∨
+			⇒ ((isAtom e2 ∧ ∃t le. e1 = Lam le ∧ e = shift_down_one_bounded (subst le (shift_up_one e2) 0)) ∨
 			   (∃e2'. M_step_inductive e2 e2' ∧ e = Apply e1 e2') ∨
 			   (∃e1'. M_step_inductive e1 e1' ∧ e = Apply e1' e2))
 Proof
 	Induct_on `M_step_inductive` >> gs[]
 QED
 
-Theorem subst_reserves_type:
-	∀Γ e t e2.
-		typeCheck_inductive Γ e t ⇒
-		typeCheck_inductive Γ (subst e (shift_up_one e2) 0) t
+Theorem type_lam_impl_type_e:
+	∀Γ e t1 t2.
+		typeChecking Γ (Lam e) (FunTy t1 t2) ⇒
+	    typeChecking (t1::Γ) e t2
 Proof
-	Induct_on `typeCheck_inductive` >> rw[]
-	>- rw[subst, typeCheck_inductive_rules]
-	>- rw[subst, typeCheck_inductive_rules, shift_up_one]
-	>- () metis_tac[subst, shift_up_one]
+	Induct_on `typeChecking` >> gs[]
+QED
+
+Theorem typeChecking_var:
+	(∀Γ n. (n < LENGTH Γ) ⇒ typeChecking Γ (Var n) (EL n Γ)) ∧
+Proof
+QED
+
+Theorem subst_reserves_type:
+	∀Γ e t1 t2 e2.
+		typeChecking (t1::Γ) e t2 ∧ typeChecking Γ e2 t1 ⇒ isAtom e2 ⇒
+		typeChecking Γ (shift_down_one_bounded (subst e (shift_up_one e2) 0)) t2
+Proof
+	Induct_on `typeChecking` >> rw[]
+	>- rw[subst, typeChecking_rules, shift_down_one_bounded]
+	>- (rw[subst, typeChecking_rules, shift_up_one, shift_down_one_bounded]
+		>- (Cases_on `e2` >> rw[])
+		>> `n - 1 < LENGTH Γ` by (Induct_on `Γ` >> simp[])
+		>> `typeChecking Γ (Var (n - 1)) (EL (n - 1) Γ)` by simp[typeChecking_rules]
+		>> Cases_on `n` >> gs[])
+	>- (rw[shift_up_one, shift_down_one_bounded, Once subst, typeChecking_rules]
+		>> Cases_on `e2` >> rw[Once subst] >> )
 QED
 
 Theorem M_preservation_2:
-	∀Γ e e' t. typeCheck_inductive Γ e t ∧ M_step_inductive e e' ⇒ typeCheck_inductive Γ e' t
+	∀Γ e e' t. typeChecking Γ e t ∧ M_step_inductive e e' ⇒ typeChecking Γ e' t
 Proof
-	Induct_on `typeCheck_inductive` >> rw[M_step_inductive_rules, typeCheck_inductive_rules]
-	>- metis_tac[lit_m_step_lit, typeCheck_inductive_rules]
-	>- metis_tac[typetag_m_step_typetag, typeCheck_inductive_rules]
-	>- metis_tac[var_m_step_var, typeCheck_inductive_rules]
-	>- (drule m_step_equal >> metis_tac[typeCheck_inductive_rules])
-	>- (drule m_step_if >> metis_tac[typeCheck_inductive_rules])
+	Induct_on `typeChecking` >> rw[M_step_inductive_rules, typeChecking_rules]
+	>- metis_tac[lit_m_step_lit, typeChecking_rules]
+	>- metis_tac[var_m_step_var, typeChecking_rules]
+	>- (drule m_step_equal >> metis_tac[typeChecking_rules])
+	>- (drule m_step_if >> metis_tac[typeChecking_rules])
 	>- (rename[`M_step_inductive (Apply e1 e2) e`] >>
 		drule m_step_apply >> rw[]
-		>- ()
-		>> metis_tac[typeCheck_inductive_rules])
-	>> metis_tac[lam_m_step_lam, typeCheck_inductive_rules]
+		>- (rename [`typeChecking Γ (Lam e) (FunTy t1 t2)`] >>
+			drule type_lam_impl_type_e >> rw[] >>
+			)
+		>> metis_tac[typeChecking_rules])
+	>> metis_tac[lam_m_step_lam, typeChecking_rules]
 QED
 
 (*
